Remove receives, fix ciu, ctx, simplify case frame

Erl_codes/weird.erl
@@ -1,0 +1,45 @@
+-module(weird).
+-compile(export_all).
+
+f() ->
+  self() ! 1,
+  self() ! 2,
+  self() ! 3,
+  receive
+    2 when 1 / 0 -> "You got me"
+  after 0 -> [receive X -> X after 0 -> "No more values" end, receive X -> X after 0 -> "No more values" end, receive X -> X after 0 -> "No more values" end]
+  end.
+
+flush() ->
+  receive
+    X -> io:format("Process ~p got: ~p~n", [self(), X]), flush()
+  after
+    0 -> ok
+  end.
+
+g(X) ->
+  case X of
+    true -> spawn(weird, slave, [self()]);
+    false -> ok
+  end,
+  receive
+    1 when false -> ok;
+    2 when false -> ok;
+    7 -> finished
+  after
+    10 -> flush(), g(false)
+  end.
+
+slave(Pid) ->
+  Pid ! 1,
+  Pid ! 2,
+  timer:sleep(10),
+  Pid ! 3,
+  Pid ! 4,
+  timer:sleep(10),
+  Pid ! 5,
+  Pid ! 6,
+  timer:sleep(10),
+  Pid ! 7.
+
+recurse() -> recurse().
